stuck since we do not have idestruct tactic

src/Carte/Wpi.lean
@@ -8,40 +8,91 @@ open Iris BI ITree
 
 section wp_itree
 
-variable {PROP : Type _} [BI PROP] [BUpd PROP]
+variable {E} {PROP : Type _} [BI PROP] [BIUpdate PROP] (H : IHandler (PROP := PROP) E)
 
 -- The definition of the weakest precondition, prior to taking the fixpoint.
-def wpiF {E R} (H : IHandler (PROP := PROP) E)
-    (wpi : LeibnizO (ITree E R) → (R → PROP) → PROP) :
-    LeibnizO (ITree E R) → (R → PROP) → PROP :=
+def wpiF {R} (wpi : ITree E R → (R → PROP) → PROP) :
+    ITree E R → (R → PROP) → PROP :=
   fun t Φ =>
     iprop(
-      |==> match t.car.unfold with
+      |==> match t.unfold with
       | ITreeF.ret r => Φ r
-      | ITreeF.tau t' => wpi ⟨t'⟩ Φ
+      | ITreeF.tau t' => wpi t' Φ
       | ITreeF.vis i k =>
           H.ihandle i
-            (fun a => wpi ⟨k a⟩ Φ)
-            (fun a => iprop(|==> wpi ⟨k a⟩ (fun _ => iprop(False))))
+            (fun a => wpi (k a) Φ)
+            (fun a => iprop(|==> wpi (k a) (fun _ => iprop(False))))
     )
-def wpiF' {E R} (H : IHandler (PROP := PROP) E)
-    (wpi : LeibnizO (ITree E R) × (R → PROP) → PROP) :
+
+-- [LeibnizO] wrapped version of wpiF
+def wpiF' {R} (wpi : LeibnizO (ITree E R) × (R → PROP) → PROP) :
     LeibnizO (ITree E R) × (R → PROP) → PROP :=
-  fun ⟨t, Φ⟩ => wpiF H (Function.curry wpi) t Φ
+  fun ⟨t, Φ⟩ => wpiF H (fun t Φ => wpi (⟨t⟩, Φ)) t.car Φ
 
-def wpi {E R} (H : IHandler (PROP := PROP) E) (t : ITree E R) (Φ : R → PROP) : PROP :=
-    bi_least_fixpoint (wpiF' H) (⟨t⟩, Φ)
+/-- Helper function for proving BIMonoPred -/
+instance {R} : OFE (LeibnizO (ITree E R) × (R → PROP) → PROP) := by
+  infer_instance
 
-theorem wpiF_mono [BI PROP] [BUpd PROP]
-    (H : IHandler (PROP := PROP) E)
-    (wp1 wp2 : LeibnizO (ITree E R) → (R → PROP) → PROP) :
+-- set_option trace.Meta.synthInstance true in
+-- instance {R} : OFE.NonExpansive (wpiF' H) where
+--   ne {n wp1 wp2} Hwp x := by
+--     sorry
+
+
+theorem wpiF_mono {R} (wp1 wp2 : ITree E R → (R → PROP) → PROP) :
     ⊢ □ (∀ t Φ, wp1 t Φ -∗ wp2 t Φ) -∗
       ∀ t Φ, wpiF H wp1 t Φ -∗ wpiF H wp2 t Φ := by
   iintro □Hwand %t %Φ Hwp
-  unfold wpiF at *
-  sorry
+  unfold wpiF
+  cases t.unfold <;> simp only
+  case ret => iexact Hwp
+  case tau t' => imod Hwp; imodintro; irevert Hwp; iexact Hwand
+  case vis i k =>
+    imod Hwp; imodintro; iapply H.ihandle_mono
+    · iintro %a Hk; iapply Hwand $$ Hk
+    · iintro !> %a Hk; imod Hk; imodintro; iapply Hwand $$ Hk
+    · iexact Hwp
 
--- theorem wpi_unfold_mask H (t : ITree E R) Φ : wpi H t Φ ⊣⊢ wpiF H (fun t Φ => wpi H t.car Φ) ⟨t⟩ Φ := by
+theorem wpiF'_mono {R} (wp1 wp2 : LeibnizO (ITree E R) × (R → PROP) → PROP) :
+    ⊢ □ (∀ t Φ, wp1 (t, Φ) -∗ wp2 (t, Φ)) -∗
+      ∀ t Φ, wpiF' H wp1 (t, Φ) -∗ wpiF' H wp2 (t, Φ) := by
+  simp [wpiF']
+  iintro □Hwand %t' %Φ Hwp
+  cases t' with | mk t =>
+    simp only
+    iapply wpiF_mono (wp1 := fun t Φ => wp1 ({ car := t }, Φ)) (wp2 := fun t Φ => wp2 ({ car := t }, Φ))
+    . iintro !> %t' %Φ' Hw; iapply Hwand $$ %⟨t'⟩, %Φ', Hw
+    . iexact Hwp
+
+/-- End of Helper -/
+
+instance {R} : BIMonoPred (λ wp_itree : LeibnizO (ITree E R) × (R → PROP) → PROP => wpiF' H wp_itree) where
+  mono_pred := by
+    iintro %Φ %Ψ %HΦ %HΨ □H %pair Hsim
+    iapply wpiF'_mono (wp1 := Φ) (wp2 := Ψ)
+    . iintro !> %t %Φ1; iapply H
+    . iexact Hsim
+  mono_pred_ne := by
+    intros Φ HΦ
+    -- unfold OFE.NonExpansive
+    sorry
+
+def wpi {E R} (H : IHandler (PROP := PROP) E) (t : ITree E R) (Φ : R → PROP) : PROP :=
+  bi_least_fixpoint (wpiF' H) (⟨t⟩, Φ)
+
+-- set_option trace.Meta.synthInstance true in
+-- theorem wpiF_ne {E R n} (H : IHandler (PROP := PROP) E)
+--     (wp1 wp2 : ITree E R → (R → PROP) → PROP) :
+--     ∀ t1 t2 (Φ1 Φ2 : R → PROP), t1 ≡{n}≡ t2 → Φ1 ≡{n}≡ Φ2 → wpiF H wp1 t1 ≡{n}≡ wpiF H wp2 t2 := by
+--   intros t1 t2 Φ1 Φ2 Ht HΦ
+--   subst Ht
+--   unfold wpiF at ⊢
+--   apply OFE.NonExpansive.ne (f := BUpd.bupd (PROP := PROP))
+
+--   iintro
+-- set_option pp.all true in
+
+-- theorem wpi_unfold_mask H (t : ITree E R) Φ : wpi H t Φ ⊣⊢ wpiF H (wpi H) t Φ := by
 --   sorry
 
 end wp_itree
